Improve error messages for reveal

Source/DafnyCore/Resolver/NameResolutionAndTypeInference/NameResolutionAndTypeInference.cs
@@ -3535,7 +3535,7 @@ namespace Microsoft.Dafny {
               var e = (ApplySuffix)expr;
               var methodCallInfo = ResolveApplySuffix(e, revealResolutionContext, true);
               if (methodCallInfo == null) {
-                reporter.Error(MessageSource.Resolver, expr.tok, "expression has no reveal lemma");
+                // error has already been reported
               } else if (methodCallInfo.Callee.Member is TwoStateLemma && !revealResolutionContext.IsTwoState) {
                 reporter.Error(MessageSource.Resolver, methodCallInfo.Tok, "a two-state function can only be revealed in a two-state context");
               } else if (methodCallInfo.Callee.AtLabel != null) {
@@ -4568,7 +4568,28 @@ namespace Microsoft.Dafny {
     }
 
     private void ReportMemberNotFoundError(IToken tok, string memberName, TopLevelDecl receiverDecl) {
+      if (memberName.StartsWith(RevealStmt.RevealLemmaPrefix)) {
+        var nameToBeRevealed = memberName[RevealStmt.RevealLemmaPrefix.Length..];
+        var members = receiverDecl is TopLevelDeclWithMembers topLevelDeclWithMembers ? GetClassMembers(topLevelDeclWithMembers) : null;
+        if (members == null) {
+          reporter.Error(MessageSource.Resolver, tok, $"member '{nameToBeRevealed}' does not exist in {receiverDecl.WhatKind} '{receiverDecl.Name}'");
+        } else if (!members.TryGetValue(nameToBeRevealed, out var member)) {
+          reporter.Error(MessageSource.Resolver, tok, $"member '{nameToBeRevealed}' does not exist in {receiverDecl.WhatKind} '{receiverDecl.Name}'");
+        } else if (member is not (ConstantField or Function)) {
+          Contract.Assert(!member.IsOpaque);
+          reporter.Error(MessageSource.Resolver, tok,
+            $"a {member.WhatKind} ('{nameToBeRevealed}') cannot be revealed; only opaque constants and functions can be revealed");
+        } else if (!member.IsOpaque) {
+          reporter.Error(MessageSource.Resolver, tok, $"{member.WhatKind} '{nameToBeRevealed}' cannot be revealed, because it is not opaque");
+        } else if (member is Function { Body: null }) {
+          reporter.Error(MessageSource.Resolver, tok,
+            $"{member.WhatKind} '{nameToBeRevealed}' cannot be revealed, because it has no body in {receiverDecl.WhatKind} '{receiverDecl.Name}'");
+        } else {
+          reporter.Error(MessageSource.Resolver, tok, $"cannot reveal '{nameToBeRevealed}'");
+        }
+      } else {
         reporter.Error(MessageSource.Resolver, tok, $"member '{memberName}' does not exist in {receiverDecl.WhatKind} '{receiverDecl.Name}'");
+      }
     }
 
     /// <summary>
@@ -5402,7 +5423,9 @@ namespace Microsoft.Dafny {
         // ----- None of the above
         if (complain) {
           if (resolutionContext.InReveal) {
-            reporter.Error(MessageSource.Resolver, expr.tok, "cannot reveal '{0}' because no constant, assert label, or requires label in the current scope is named '{0}'", expr.Name);
+            reporter.Error(MessageSource.Resolver, expr.tok,
+              "cannot reveal '{0}' because no revealable constant, function, assert label, or requires label in the current scope is named '{0}'",
+              expr.Name);
           } else {
             reporter.Error(MessageSource.Resolver, expr.tok, "unresolved identifier: {0}", name);
           }
